#+TITLE: Intermediate Value Theorem
#+LATEX_HEADER: \usepackage{mathtools}

* Definition

The Intermediate Value Theorem (IVT) states the following:

Let \( f: [a, b] \to \mathbb{R} \) be some function continuous on the interval \( [a, b] \), with \( f(a) = A \) and \( f(b) = B \). Let \( C \in \mathbb{R} \) be such that \( min\{A, \ B\} < C < max\{A, \ B\} \), then:

\[
\exists c \in [a, b] \ s.t. \ f(c) = C
\]

And:

\[
S = \{x : x \in [a, b], f(z) \le C \ \forall z \in [a, x] \}
\]
\[
c = \sup\{S\}
\]

* Proof

Suppose WLOG that \( f(a) < f(b) \). Note since \( S \) is bounded above by \( b \) and nonempty, it must have a supremum by the completeness property of the reals, hence \( c \) is defined.

** Case 1

   Now suppose \( f(c) < C \implies C - f(c) = \epsilon > 0 \). Now since \( f \) is continuous on \( [a, b] \):

   \[
   \exists \delta > 0 \ s.t. \ x \in (c - \delta, c + \delta) \implies \ |f(c) - f(x)| < \epsilon
   \]

   Now consider any :

   \[
   c^* \in (c, c + \delta) 
   \]

   Note since \( |f(c^*) - f(x)| < \epsilon \implies f(c^*) < f(c) + \epsilon = C \) there is no \( c^* \) such that \( f(c^*) > C \), hence all \( c^* \) are in \( S \), but this is a contradiction as their memebership in the set would mean

   \[
   c \ne sup\{S\}
   \]

   So we can conclude that our assumption: \( f(c) < C \) is false.

** Case 2
   Alternatively, suppose \( f(c) > C \implies f(c) - C = \epsilon > 0 \). By continuity:

   \[
   \exists \delta > 0 \ s.t. \ x \in (c - \delta, c + \delta) \implies \ |f(c) - f(x)| < \epsilon
   \]

   Now choose \( c' = c - \frac{\epsilon}{2} \). We prove the above supposition to be false by considering the membership of \( c' \) to \( S \). We know from the membership predicates of \( S \) that \( c \) cannot be in \( S \). Suppose:

   \[
   c' \not \in S \implies \forall x \ge c', \ x \not \in C \implies c' \text{ is an upper bound of } S
   \]

   But that would contradict the definition of \( c \) being the least upper bound of \( S \), hence we must have \( c' \in S \).

   \[ 
   c' \in S \implies f(c') \le C
   \]

   But we know from continuity: \( f(c) - f(c') \le \epsilon \)

   \begin{align}
   & \implies f(c) - f(c') \le f(c) - C\\
   & \implies C \le f(c')\\
   & \implies c' \not \in S
   \end{align}

   Which again arrives us at a contradiction, hence the statement \( f(c) > C \) is false.

** Synthesis

   Given that the statements \( f(c) > C \) and \( f(c) < C \) are both false, we deduce that \( f(c) = C \) which proves the theorem.




